break things more

LeanSAT/Model/PropAssn.lean
@@ -140,14 +140,55 @@ theorem agreeOn_setMany_compl (xs : Finset ν) (τ')
 def map (f : ν₂ → ν₁) (τ : PropAssignment ν₁) : PropAssignment ν₂ :=
   τ ∘ f
 
-@[simp] theorem app_map : map f τ v = τ (f v) := rfl
+@[simp] theorem get_map : map f τ v = τ (f v) := rfl
+
+@[simp] theorem map_set [DecidableEq ν₁] [DecidableEq ν₂] (f : ν₂ → ν₁) (τ) (finj : f.Injective) :
+    map f (set τ (f v) b) = set (map f τ) v b := by
+  unfold map; unfold set; ext; simp [finj.eq_iff]
 
 def pmap {P : ν₂ → Prop} [DecidablePred P]
-    (f : { v : ν₂ // P v } → ν₁) (τ : PropAssignment ν₁) : PropAssignment ν₂ :=
+    (f : Subtype P → ν₁) (τ : PropAssignment ν₁) : PropAssignment ν₂ :=
   fun v =>
     if h : P v then τ (f ⟨v,h⟩) else false
 
-@[simp] theorem pmap_subtype_val {P : ν₂ → Prop} [DecidablePred P]
-    (f : { v : ν₂ // P v } → ν₁) (τ) (x : Subtype P)
+@[simp]
+theorem pmap_subtype_val {P : ν₂ → Prop} [DecidablePred P]
+    (f : Subtype P → ν₁) (τ) (x : Subtype P)
   : pmap f τ (Subtype.val x) = τ (f x) := by
   simp [pmap, Subtype.property]
+
+@[simp]
+theorem get_pmap {P : ν₂ → Prop} [DecidablePred P]
+    (f : Subtype P → ν₁) (τ) (x : ν₂) (h : P x)
+  : pmap f τ x = τ (f ⟨x,h⟩) := by
+  simp [pmap,h]
+
+@[simp]
+theorem pmap_map {P : ν₂ → Prop} [DecidablePred P]
+    (f : {v : ν₂ // P v} → ν₁) (g : ν₁ → ν₀) (τ)
+  : pmap f (map g τ) = pmap (g ∘ f) τ := rfl
+
+theorem pmap_pmap {P : ν₂ → Prop} [DecidablePred P] {Q : ν₁ → Prop} [DecidablePred Q]
+    (f : Subtype P → ν₁) (g : Subtype Q → ν₀) (τ : PropAssignment ν₀)
+  : pmap f (pmap g τ) =
+      pmap
+        (P := fun v2 => ∃ h, Q (f ⟨v2,h⟩))
+        (fun ⟨v2,h⟩ => g ⟨ f ⟨v2,h.1⟩, h.2⟩)
+        τ
+  := by
+  ext v2
+  simp [pmap]; split <;> simp_all
+
+
+def preimage [Fintype ν₁] [DecidableEq ν₂] (f : ν₁ ↪ ν₂) (τ : PropAssignment ν₁)
+    : PropAssignment ν₂ :=
+  pmap (fun ⟨v2,h⟩ => (Finset.mapEquiv Finset.univ f).symm ⟨v2,h⟩) τ
+
+theorem get_preimage [Fintype ν₁] [DecidableEq ν₂] (f : ν₁ ↪ ν₂) {τ v v'}
+    : v = f.1 v' → (preimage f τ) v = τ v' := by
+  rintro rfl; simp [preimage, pmap]
+
+@[simp]
+theorem map_preimage [Fintype ν₁] [DecidableEq ν₂] (f : ν₁ → ν₂) (f') (τ)
+    : f = f'.1 → map f (preimage f' τ) = τ := by
+  rintro rfl; ext v1; simp [preimage]
